spec/SQS.thy
@@ -2,8 +2,6 @@ theory SQS
   imports Main "./Queue"
 begin
 
-datatype ClientId = ClientId nat
-
 datatype 'a SQSRequest
   = Send 'a
   | Receive nat
@@ -12,19 +10,20 @@ datatype 'a SQSRequest
 datatype 'a SQSResponse
   = Returned "(MessageId \<times> 'a) list"
 
-record 'a SQSState =
+record ('proc, 'a) SQSState =
   queue :: "'a Queue"
-  request :: "('a SQSRequest) option"
-  response :: "('a SQSResponse) option"
+  request :: "('proc \<times> 'a SQSRequest) option"
+  response :: "('proc \<times> 'a SQSResponse) option"
 
-definition initialSQSState :: "'a SQSState" where
+definition initialSQSState :: "('proc, 'a) SQSState" where
   "initialSQSState = \<lparr> queue = Queue.empty, request = None, response = None \<rparr>"
 
-fun SQS_step :: "'a SQSState \<Rightarrow> 'a SQSState" where
+fun SQS_step :: "('proc, 'a) SQSState \<Rightarrow> ('proc, 'a) SQSState" where
   "SQS_step st = (case request st of
-    Some (Send v) \<Rightarrow> st \<lparr> queue := insert (queue st) v, response := None \<rparr>
-  | Some (Receive n) \<Rightarrow> st \<lparr> response := Some (Returned (pick (queue st) n)) \<rparr>
-  | Some (Delete m) \<Rightarrow> st \<lparr> queue := delete (queue st) m, response := None \<rparr>
+    Some ((_, Send v)) \<Rightarrow> st \<lparr> queue := insert (queue st) v, response := None \<rparr>
+  | Some ((proc, Receive n)) \<Rightarrow> st \<lparr> response := Some ((proc, Returned (pick (queue st) n))) \<rparr>
+  | Some ((_, Delete m)) \<Rightarrow> st \<lparr> queue := delete (queue st) m, response := None \<rparr>
+  | _ \<Rightarrow> st
   ) \<lparr> request := None \<rparr>"
 
 end
